LeanSubst/Expanded.lean
@@ -6,8 +6,22 @@ import LeanSubst.Class
 namespace LeanSubst
 
 universe u1 u2 u3
-variable {S : Type u1} {T T1 T2 : Type u2} {U : Type u3}
+variable {S : Type u1} {T T1 T2 T3 : Type u2} {U : Type u3}
 variable {V : List (Type u2)}
+
+
+@[grind =_]
+theorem RenVec.get_eta1 {r : RenVec [T1]} : r = (r.get T1 0, .unit) := sorry
+
+@[grind =_]
+theorem RenVec.get_eta2 {r : RenVec [T1, T2]} : r = (r.get T1 0, r.get T2 1, .unit) := sorry
+
+@[grind =_]
+theorem SubstVec.get_eta1 {σ : SubstVec [T1]} : σ = (σ.get T1 0, .unit) := sorry
+
+@[grind =_]
+theorem SubstVec.get_eta2 {σ : SubstVec [T1, T2]} : σ = (σ.get T1 0, σ.get T2 1, .unit) := sorry
+
 
 -- @[simp]
 -- theorem subst_tuple_eta1 [SubstMap S [T]] {s : S} {σ : List.Tuple Subst [T]} : s[σ,] = s[σ.1] := by
